revising and document Transcript API; removing preorder polymorphism in repr

src/tls/HSL.Transcript.fsti
@@ -1,15 +1,48 @@
-module HSL.Transcript
+(*
+  Copyright 2015--2019 INRIA and Microsoft Corporation
 
-(* Main issue:
+  Licensed under the Apache License, Version 2.0 (the "License");
+  you may not use this file except in compliance with the License.
+  You may obtain a copy of the License at
 
-   We need a way to add messages to the transcript without setting the
-   hash alg.
+    http://www.apache.org/licenses/LICENSE-2.0
 
-   Once the hash alg is set, we need to "catch up" and hash the
-   unhashed messages accumulated so far.
+  Unless required by applicable law or agreed to in writing, software
+  distributed under the License is distributed on an "AS IS" BASIS,
+  WITHOUT WARRANTIES OR CONDITIONS OF ANY KIND, either express or implied.
+  See the License for the specific language governing permissions and
+  limitations under the License.
 
-   For this, we need some auxiliary state.
+  Authors: C. Fournet, T. Ramananandro, A. Rastogi, N. Swamy
 *)
+module HSL.Transcript
+//Should this be called MITLS.TranscriptHash?
+
+(* Summary:
+
+   This module provides support for the transcript hash,
+   as described in:
+
+   https://tlswg.org/tls13-spec/draft-ietf-tls-tls13.html#rfc.section.4.4.1
+
+   Concretely, it is just an encapsulation of
+   EverCrypt.Hash.Incremental, maintaining an incremental hash of a
+   sequence of messages, as requested by its callers. At any point,
+   the current value of the hash can be extracted into a
+   caller-provided buffer.
+
+   However, abstractly, it constructs an (erased) "transcript", a
+   protocol-version-specific sequence of messages, maintaining an
+   invariant that correlates the transcript with the state of the
+   incremental hash.
+
+   The main proof provided by the module is an injectivity property,
+   based on a collision-resistance property of the underlying hashing
+   algorithm: agreement on hashed values implies agreement on the
+   transcript.
+*)
+
+
 open FStar.Integers
 open FStar.HyperStack.ST
 module List = FStar.List.Tot
@@ -24,6 +57,7 @@ module HSM13 = Parsers.Handshake13
 module PV = Parsers.ProtocolVersion
 module LP = LowParse.Low.Base
 module IncHash = EverCrypt.Hash.Incremental
+module HashDef = Spec.Hash.Definitions
 
 module R = MITLS.Repr
 module R_HS = MITLS.Repr.Handshake
@@ -34,23 +68,89 @@ module CH = Parsers.ClientHello
 module R_SH = MITLS.Repr.ServerHello
 module SH = Parsers.ServerHello
 
+
+//TODO: move to a separate module
+let repr_hs12 (b:R.slice) =
+  R.repr_p _ b HSM12.handshake12_parser
+
+//TODO: move to a separate module
+let repr_hs13 (b:R.slice) =
+  R.repr_p _ b HSM13.handshake13_parser
+
 type bytes = FStar.Seq.seq uint_8
 
-type alg = Spec.Hash.Definitions.hash_alg
-
-
+/// `hs_ch` and `hs_sh`: Abbreviations for handshake messages that
+/// hold client and server hellos, respectively
 let hs_ch = ch:HSM.handshake{HSM.M_client_hello? ch}
 let hs_sh = sh:HSM.handshake{HSM.M_server_hello? sh}
+
+/// `is_hrr`: For now, we assume the existence of a pure function to
+/// decide if a server-hello message is a hello-retry-request (hrr)
 // assume
 val is_hrr (sh:hs_sh) : bool
 
+/// `hello_retry_request`: The type of HRR messages
 inline_for_extraction
-let hello_retry_request : Type0 = 
+let hello_retry_request : Type0 =
   s:hs_sh { is_hrr s }
 
+/// `retry`: a pair of a client hello and hello retry request
 type retry =
   hs_ch
   & hello_retry_request
+
+/// `client_hello_has_psk`: A client hello has a pre-shared key if
+///    that mode appears in one of its extensions
+let client_hello_has_psk (ch:CH.clientHello) =
+  exists (ext:_).
+    List.memP ext Parsers.ClientHello.(ch.extensions) /\
+    Parsers.ClientHelloExtension.CHE_pre_shared_key? ext /\
+    True (* what else do we need? e.g., that it has as many binders as ids? *)
+
+/// `nego_version`: This is to be provided eventually by a refactoring
+/// of the Negotiation module.
+// assume
+val nego_version (ch:hs_ch)
+                 (sh:hs_sh)
+       : PV.protocolVersion
+
+/// `max_transcript_size` and `max_message_size`:
+///
+/// Some complications arise from the maximum size of transcript
+/// hashes, since the EverCrypt API imposes a maximum number of bytes
+/// that can be accumulated in an incremental hash (2^61 or 2^125,
+/// depending on the choice of algorithm). Given that each message is
+/// bounded in size by `max_message_size` (2^24), we conservatively
+/// bound the size of the transcript (`max_transcript_size`) to 2^32
+/// messages so that client code an easily track its length with a
+/// u32.
+///
+/// Note, `max_transcript_size` should be at least
+///  max (handshake12_parser_kind.parser_kind_high,
+///       handshake13_parser_kind.parser_kind_high,
+///       handshake_parser_kind.parser_kind_high)
+unfold
+let max_message_size = normalize_term (pow2 24)
+
+unfold
+let max_transcript_size : pos = normalize_term (pow2 32)
+
+
+/// This lemma proves that the maximum size in bytes of a transcript
+/// is smaller than the bound imposed by the Hash API
+let max_message_size_lt_max_input_length (a: HashDef.hash_alg)
+  : Lemma
+    ((max_transcript_size + 4) * max_message_size < HashDef.max_input_length a)
+    [SMTPat (Spec.Hash.Definitions.max_input_length a)]
+  = assert_norm ((max_transcript_size + 4) * max_message_size < pow2 61);
+    assert_norm ((max_transcript_size + 4) * max_message_size < pow2 125)
+
+/// Move to the FStar.List library?
+let bounded_list 'a n = l:list 'a{List.length l < n}
+
+(*** Main state machine ***)
+
+(** STATES **)
 
 /// `transcript_t`: Transcript for 1.2 and 1.3 have a shared prefix
 /// and then fork to version-specific message types
@@ -59,96 +159,165 @@ type retry =
 ///   is negotiated and so does not contain either HSM12 or HSM13
 ///   messages. The three types are disjoint and parsed independently.
 ///
-/// Does not yet cover Hello retry request (?)
-///
-/// Question: How much refinement do we need in this type?  e.g.,
-/// number and shape of the h-prefix of the last two cases
-
-unfold
-let max_transcript_size : pos = 15
-
-let bounded_list 'a n = l:list 'a{List.length l < n}
-
-let can_extend_bounded_list #a #n (l:bounded_list a n) = List.length l + 1 < n
-
-open Parsers.ClientHello
-let client_hello_has_psk (ch:CH.clientHello) =
-  exists (ext:_). 
-    List.memP ext ch.extensions /\
-    Parsers.ClientHelloExtension.CHE_pre_shared_key? ext /\
-    True (* what else do we need? e.g., that it has as many binders as ids? *)
-
+/// Further, each of the first two states have a variant in support of
+/// hello-retry requests. The transcript hash records the full
+/// transcript, including the retry, if any. Note, the standard
+/// forbids multiple retries.
 noeq
 type transcript_t =
-  | Start: retried:option retry ->
-           transcript_t
+  | Start:
+      retried:option retry ->
+      transcript_t
 
-  | Hello: retried:option retry ->
-           ch:hs_ch ->
-           transcript_t
+  | Hello:
+      retried:option retry ->
+      ch:hs_ch ->
+      transcript_t
 
-  | Transcript12: ch:hs_ch ->
-                  sh:hs_sh -> //Should prescribe the protocol version
-                  rest:bounded_list HSM12.handshake12 max_transcript_size ->
-                  transcript_t
+  | Transcript12:
+      ch:hs_ch ->
+      sh:hs_sh{nego_version ch sh == PV.TLS_1p2} ->
+      rest:bounded_list HSM12.handshake12 max_transcript_size ->
+      transcript_t
 
-  | Transcript13: retried:option retry ->
-                  ch:hs_ch ->
-                  sh:hs_sh -> //Should prescribe the protocol version
-                  rest:bounded_list HSM13.handshake13 max_transcript_size -> //but requires a dependence on Nego
-                  transcript_t
-      
-let transcript_n (n:nat{n < max_transcript_size}) =
-  t:transcript_t{
+  | Transcript13:
+      retried:option retry ->
+      ch:hs_ch ->
+      sh:hs_sh{nego_version ch sh == PV.TLS_1p3} ->
+      rest:bounded_list HSM13.handshake13 max_transcript_size ->
+      transcript_t
+
+/// `transcript_size`: the size of a transcript is the length of its
+/// protocol-specific suffix
+let transcript_size (t:transcript_t) =
     match t with
     | Start _
-    | Hello _ _ -> True
-    | Transcript12 _ _ rest -> List.length rest < n
-    | Transcript13 _ _ _ rest -> List.length rest < n
-  }
+    | Hello _ _ -> 0
+    | Transcript12 _ _ rest -> List.length rest
+    | Transcript13 _ _ _ rest -> List.length rest
+
+/// `extensible`: a transcript is extensible if it is smaller than
+/// `max_transcript_size`
+let extensible (t:transcript_t) = transcript_size t < max_transcript_size - 1
+let ext_transcript_t = t:transcript_t{extensible t}
 
 /// `transcript_bytes`: The input of the hash algorithm computed by
 /// concatenated the message formatting of the messages
-///
-/// Note, new messages are cons'd to the front of the transcript so
-/// formatting is a fold right. This is convenient here, but is
-/// potentially contentious since other parts of the code
-/// use snoc
-///
-/// Note: we want this to be in Tot
+val transcript_bytes (t:transcript_t)
+  : GTot (b: bytes {
+       Seq.length b <= (max_transcript_size + 4) * max_message_size
+    })
 
-// should be at least 
-//   max (handshake12_parser_kind.parser_kind_high,
-//        handshake13_parser_kind.parser_kind_high,
-//        handshake_parser_kind.parser_kind_high)
-unfold // to recover Z3 linearity
-let max_message_size = 16777219 
+(** TRANSITIONS **)
 
-val transcript_bytes (t:transcript_t) 
-: GTot (b: bytes { 
-       Seq.length b <= (max_transcript_size + 4) * max_message_size 
-  })
+/// `extend_with_hsm`: The main transition function
+///
+///    Dictates which next state to transition to (if any) from a
+///    given transcript and a message
+let transition_hsm
+      (t:transcript_t)
+      (m:HSM.handshake)
+  : GTot (option transcript_t)
+  = match t, m with
+    | Start retry, HSM.M_client_hello ch ->
+      //Missing: consistency between retry and ch
+      Some (Hello retry m)
+
+    | Hello retry ch, HSM.M_server_hello sh ->
+      if None? retry
+      && is_hrr m
+      then None
+      else
+        begin
+        match nego_version ch m, retry with
+        | PV.TLS_1p2, None ->
+          Some (Transcript12 ch m [])
+
+        | PV.TLS_1p3, _ ->
+          Some (Transcript13 retry ch m [])
+
+        | _ -> None
+        end
+
+    | _ ->
+      None
+
+/// `transition_hrr`:
+///    An auxiliary transition function, specific to TLS1.3
+///    that handles hello-retry requests
+let transition_hrr
+       (t:transcript_t)
+       (ch:HSM.handshake)
+       (sh:HSM.handshake) =
+  match t, ch, sh with
+  | Start None, HSM.M_client_hello _, HSM.M_server_hello _ ->
+    if is_hrr sh
+    then Some (Start (Some (ch, sh)))
+    else None
+  | _ ->
+    None
+
+/// `transition_hsm12`:
+///    An auxiliary transition function, specific to TLS1.2
+///    It only enforces the length constraint on the suffix
+let transition_hsm12 (t:ext_transcript_t) (m:HSM12.handshake12)
+  : option transcript_t
+  = match t with
+    | Transcript12 ch sh rest ->
+      List.append_length rest [m];
+      Some (Transcript12 ch sh (List.snoc (rest, m)))
+
+    | _ -> None
+
+/// `transition_hsm13`:
+///    An auxiliary transition function, specific to TLS1.3
+///    It only enforces the length constraint on the suffix
+let transition_hsm13 (t:ext_transcript_t) (m:HSM13.handshake13)
+  : option transcript_t
+  = match t with
+    | Transcript13 retry ch sh rest ->
+      List.append_length rest [m];
+      Some (Transcript13 retry ch sh (List.snoc (rest, m)))
+
+    | _ -> None
+
+(*** Concrete state and transitions ***)
 
 
 /// `state`: Abstract state of the module
 ///
 /// It maintains the transcript in mutable state.
 ///
-/// We may need a way to free the state also
-val state (a:alg) : Type0
+/// We may need a way to free the state also, although if it is
+/// allocated in a connection-granularity region, it will be reclaimed
+/// along with that region.
+val state (a:HashDef.hash_alg) : Type0
 
-val invariant (#a: _) (s:state a) (t:transcript_t) (h:HS.mem) : Type0  
+/// `invariant s t h`: Relates the state of the module (i.e., the
+/// state of the underlying incremental hash) to the a particular
+/// transcript
+val invariant (#a: _) (s:state a) (t:transcript_t) (h:HS.mem) : Type0
 
+/// `footprint`: Abstract memory footprint
 val footprint (#a:_) (s:state a) : GTot B.loc
 
-val elim_invariant (#a: _) (s:state a) (t:transcript_t) (h:HS.mem) 
-  : Lemma 
+/// `elim_invariant`: One way to eliminate the invariant is simply to
+///  recover that the memory footprint of the module is used in the
+///  memory state `h`. Withouth this, it is not possible to prove that
+///  a freshly allocated location doesn't interfere with the abstract
+///  footprint of this module.
+val elim_invariant (#a: _) (s:state a) (t:transcript_t) (h:HS.mem)
+  : Lemma
     (requires invariant s t h)
     (ensures B.loc_not_unused_in h `B.loc_includes` footprint s)
 
+/// `region_of`: The internal state of the module is allocated in a
+/// user-provided region
 val region_of (#a: _) (s:state a)
   : GTot HS.rid
 
+/// `frame_invariant`: The invariant is maintained across
+/// footprint-preserving heap modifications
 val frame_invariant (#a:_) (s:state a) (t: transcript_t) (h0 h1:HS.mem) (l:B.loc)
   : Lemma
     (requires
@@ -160,16 +329,15 @@ val frame_invariant (#a:_) (s:state a) (t: transcript_t) (h0 h1:HS.mem) (l:B.loc
     [SMTPat (invariant s t h1);
      SMTPat (B.modifies l h0 h1)]
 
-/// `create`:
+/// `create`: Allocating a new instance of the transcript hash
 ///
 ///   -- Caller provides a region `r` in which to allocate a
 ///      transcript instance
 ///
 ///   -- The instance is allocated in fresh state (so `modifies none`)
 ///
-///   -- The transcript's initial state is empty and the hash alg is
-///      not chosen yet
-val create (r:Mem.rgn) (a:alg)
+///   -- The transcript's initial state is empty
+val create (r:Mem.rgn) (a:HashDef.hash_alg)
   : ST (state a & Ghost.erased transcript_t)
        (requires fun _ -> True)
        (ensures fun h0 (s, tx) h1 ->
@@ -181,147 +349,125 @@ val create (r:Mem.rgn) (a:alg)
          B.modifies B.loc_none h0 h1 /\
          B.fresh_loc (footprint s) h0 h1)
 
-unfold
-let extend_hash_pre_common
-  #a
-  (s:state a)
-  (#rrel #rel: _) (#b:LP.slice rrel rel) (#x:_) (r:R.repr x b)
-  (t:transcript_t)
-  (h:HS.mem)
-  = invariant s t h /\
-    R.valid r h /\
-    B.loc_disjoint (B.loc_buffer LP.(b.base)) (footprint s)
+(** CONCRETE STATE TRANSITIONS **)
 
+/// `extend_pre_common`: Every state transition
+/// has some basic requirements
+///   -- state machine invariant
+///   -- validity of message representations
+///   -- disjointness of machine state and representation state
+///   -- extensibility of the transcript
 unfold
-let extend_hash_post_common
-  #a
-  (s:state a)
-  (t:transcript_t)
-  (h0 h1:HS.mem)
+let extend_pre_common
+  #a (s:state a)
+  #t (#b:R.slice) (r:R.repr t b)
+  (tx:transcript_t) (h:HS.mem)
+  = invariant s tx h /\
+    R.valid r h /\
+    B.loc_disjoint (B.loc_buffer LP.(b.base)) (footprint s) /\
+    extensible tx
+
+/// `extend_hash_post_common`: Every state transition
+/// has some basic guarantees
+///   -- state machine invariant
+///   -- mutates only the state machine's footprint
+unfold
+let extend_post_common
+  #a (s:state a) (t:transcript_t) (h0 h1:HS.mem)
   = invariant s t h1 /\
     B.modifies (footprint s) h0 h1
 
-// assume 
-val nego_version (ch:CH.clientHello)
-                 (sh:SH.serverHello)
-       : PV.protocolVersion
-
-let extend_with_hsm 
-      (t:transcript_t)
-      (m:HSM.handshake)
-  : GTot (option transcript_t)
-= match t, m with
-  | Start retry, HSM.M_client_hello ch ->
-    //Missing: consistency between retry and ch
-    Some (Hello retry m)
-
-  | Hello retry ch, HSM.M_server_hello sh ->
-    if None? retry
-    && is_hrr m
-    then None
-    else
-      begin
-      match nego_version 
-             (HSM.M_client_hello?._0 ch)
-             sh,
-            retry
-      with
-      | PV.TLS_1p2, None ->
-        Some (Transcript12 ch m [])
-
-      | PV.TLS_1p3, _ ->
-        Some (Transcript13 retry ch m [])
-
-      | _ -> None
-      end
-
-  | _ ->
-    None
-
-let extend_with_hsm12 (t:transcript_n (max_transcript_size - 1)) (m:HSM12.handshake12)
-  : option transcript_t
-  = match t with
-    | Transcript12 ch sh rest ->
-      List.append_length rest [m];
-      Some (Transcript12 ch sh (List.snoc (rest, m)))
-  
-    | _ -> None
-
-
-let extend_with_hsm13 (t:transcript_n (max_transcript_size - 1)) (m:HSM13.handshake13)
-  : option transcript_t
-  = match t with
-    | Transcript13 retry ch sh rest ->
-      List.append_length rest [m];
-      Some (Transcript13 retry ch sh (List.snoc (rest, m)))
-  
-    | _ -> None
-
-val extend_hash_hsm
+/// `extend_hsm`: The main transition
+///    - the state evolves according to `transition_hsm`
+val extend_hsm
   (#a:_) (s:state a)
-  (#p #q: _) (#b:LP.slice p q) (r:R_HS.repr b)
-  (tx:G.erased (transcript_n (max_transcript_size - 1)))
-  : Stack (G.erased transcript_t)
-       (requires fun h ->
-         let tx = G.reveal tx in
-         extend_hash_pre_common s r tx h /\
-         Some? (extend_with_hsm tx (R.value r)))
-       (ensures fun h0 tx' h1 ->
-         let tx' = G.reveal tx' in
-         tx' == Some?.v (extend_with_hsm (G.reveal tx) (R.value r)) /\
-         extend_hash_post_common s tx' h0 h1)
-
-//TODO: move to a separate module
-let repr_hs12  (#rrel #rel: _) (b:LP.slice rrel rel) =
-  R.repr_p _ b HSM12.handshake12_parser
-
-val extend_hash_hsm12
-  (#a:_) (s:state a)
-  (#p #q: _) (#b:LP.slice p q) (r:repr_hs12 b)
-  (tx:G.erased (transcript_n (max_transcript_size - 1)))
+  (#b:R.slice) (r:R_HS.repr b)
+  (tx:G.erased transcript_t)
   : Stack (G.erased transcript_t)
     (requires fun h ->
       let tx = G.reveal tx in
-      extend_hash_pre_common s r tx h /\
-      Some? (extend_with_hsm12 tx (R.value r)))
+      extend_pre_common s r tx h /\
+      Some? (transition_hsm tx (R.value r)))
     (ensures fun h0 tx' h1 ->
       let tx = G.reveal tx in
       let tx' = G.reveal tx' in
-      tx' == Some?.v (extend_with_hsm12 tx (R.value r)) /\
-      extend_hash_post_common s tx' h0 h1)
+      tx' == Some?.v (transition_hsm tx (R.value r)) /\
+      extend_post_common s tx' h0 h1)
 
-
-//TODO: move to a separate module
-let repr_hs13  (#rrel #rel: _) (b:LP.slice rrel rel) =
-  R.repr_p _ b HSM13.handshake13_parser
-
-val extend_hash_hsm13
+/// `extend_hsm12`: Append to Transcript12
+///    - the state evolves according to `transition_hsm12`
+val extend_hsm12
   (#a:_) (s:state a)
-  (#p #q: _) (#b:LowParse.Low.Base.slice p q) (r:repr_hs13 b)
-  (tx:G.erased (transcript_n (max_transcript_size - 1)))
+  (#b:R.slice) (r:repr_hs12 b)
+  (tx:G.erased transcript_t)
   : Stack (G.erased transcript_t)
     (requires fun h ->
       let tx = G.reveal tx in
-      extend_hash_pre_common s r tx h /\
-      Some? (extend_with_hsm13 tx (R.value r)))
+      extend_pre_common s r tx h /\
+      Some? (transition_hsm12 tx (R.value r)))
     (ensures fun h0 tx' h1 ->
-      let tx = G.reveal tx in       
+      let tx = G.reveal tx in
       let tx' = G.reveal tx' in
-      tx' == Some?.v (extend_with_hsm13 tx (R.value r)) /\
-      extend_hash_post_common s tx' h0 h1)
+      tx' == Some?.v (transition_hsm12 tx (R.value r)) /\
+      extend_post_common s tx' h0 h1)
 
+/// `extend_hsm13`: Append to Transcript13
+///    - the state evolves according to `transition_hsm13`
+val extend_hsm13
+  (#a:_) (s:state a)
+  (#b:R.slice) (r:repr_hs13 b)
+  (tx:G.erased transcript_t)
+  : Stack (G.erased transcript_t)
+    (requires fun h ->
+      let tx = G.reveal tx in
+      extend_pre_common s r tx h /\
+      Some? (transition_hsm13 tx (R.value r)))
+    (ensures fun h0 tx' h1 ->
+      let tx = G.reveal tx in
+      let tx' = G.reveal tx' in
+      tx' == Some?.v (transition_hsm13 tx (R.value r)) /\
+      extend_post_common s tx' h0 h1)
+
+/// `extend_ch_with_psk`:
+///
+///    This is a specialized transition used by the server to process
+///    client hello's with pre-shared key binders.
+///
+///    See https://tlswg.org/tls13-spec/draft-ietf-tls-tls13.html#rfc.section.4.2.11
+///
+///    Broadly, the server selects a particular PSK binder to validate.
+///
+///    Validation involves checking the hash of the transcript up to
+///    the truncated client hello under a PSK binder key. Note, this
+///    may be more than just the truncated client hello, since the
+///    transcript may als include a hello-retry request.
+///
+///    This function does the following:
+///
+///      - truncates the client hello (until just before the first PSK
+///        binder)
+///
+///      - extends the transcript hash with the truncation, extracts
+///        that hash to a freshly allocation on the stack (in the
+///        caller's stack frame; note the `StackInline`)
+///
+///      - then extends the transcript hash to with the suffix of the
+///        client hello (i.e., all the binders excluded by the truncation)
+///
+///      - and correspondingly transitions the state machine to
+///        include the entire client hello
 val extend_ch_with_psk
   (#a:_) (s:state a)
-  (#p #q: _) (#b:LowParse.Low.Base.slice p q) (r:R_HS.repr b)
+  (#b:R.slice) (r:R_HS.repr b)
   (tx:G.erased transcript_t)
-  : StackInline 
+  : StackInline
       (Hacl.Hash.Definitions.hash_t a &
        G.erased transcript_t)
     (requires fun h ->
       let tx = G.reveal tx in
       let hs = R.value r in
-      extend_hash_pre_common s r tx h /\
-      Start? tx /\         
+      extend_pre_common s r tx h /\
+      Start? tx /\
       HSM.M_client_hello? hs /\
       client_hello_has_psk (HSM.M_client_hello?._0 hs))
     (ensures fun h0 (hash, tx') h1 ->
@@ -330,49 +476,41 @@ val extend_ch_with_psk
       B.fresh_loc (B.loc_buffer hash) h0 h1 /\
       B.live h1 hash /\
       tx' == Hello (Start?.retried tx) (R.value r) /\
-      extend_hash_post_common s tx' h0 h1)
+      extend_post_common s tx' h0 h1)
 
-let extend_with_hrr 
-       (t:transcript_t)
-       (ch:HSM.handshake)
-       (sh:HSM.handshake) =
-  match t, ch, sh with       
-  | Start None, HSM.M_client_hello _, HSM.M_server_hello _ ->
-    if is_hrr sh
-    then Some (Start (Some (ch, sh)))
-    else None
-  | _ ->
-    None
-    
+/// `extend_hrr`: Hello retry requests
+///     See https://tlswg.org/tls13-spec/draft-ietf-tls-tls13.html#rfc.section.4.1.4
+///  Transitions according to `transition_hrr`
 val extend_hrr
   (#a:_) (s:state a)
-  (#p #q:_) (#b:LP.slice p q) (r_ch:R_HS.repr b)
-  (#p' #q':_) (#b':LP.slice p' q') (r_sh:R_HS.repr b')  
+  (#b:R.slice) (r_ch:R_HS.repr b)
+  (#b':R.slice) (r_sh:R_HS.repr b')
   (tx:G.erased transcript_t)
   : Stack (G.erased transcript_t)
-      (requires fun h ->
-         let tx = G.reveal tx in
-         extend_hash_pre_common s r_sh tx h /\
-         Some? (extend_with_hrr tx (R.value r_ch) (R.value r_sh)))
-       (ensures fun h0 tx' h1 ->                                     
-         let tx = G.reveal tx in
-         let tx' = G.reveal tx' in
-         tx' == Some?.v (extend_with_hrr tx (R.value r_ch) (R.value r_sh)) /\
-         extend_hash_post_common s tx' h0 h1)         
+    (requires fun h ->
+      let tx = G.reveal tx in
+      extend_pre_common s r_sh tx h /\
+      Some? (transition_hrr tx (R.value r_ch) (R.value r_sh)))
+    (ensures fun h0 tx' h1 ->
+      let tx = G.reveal tx in
+      let tx' = G.reveal tx' in
+      tx' == Some?.v (transition_hrr tx (R.value r_ch) (R.value r_sh)) /\
+      extend_post_common s tx' h0 h1)
 
+(*** Extracting hashes and injectivity ***)
 
-let max_message_size_lt_max_input_length (a: alg) : Lemma
-  (max_transcript_size * max_message_size < Spec.Hash.Definitions.max_input_length a)
-  [SMTPat (Spec.Hash.Definitions.max_input_length a)] 
- =
-  assert_norm (max_transcript_size * max_message_size < pow2 61);
-  assert_norm (max_transcript_size * max_message_size < pow2 125)
-
+/// `extract_hash`:
+///
+///   At any point, we can extract the current state of thea
+///   incremental hash into a user-provided buffer to store the tag
+///
+///   The post-condition ensures that the tag contains a hash of the
+///   transcript bytes
 val extract_hash
-  (#a:alg) (s:state a)
+  (#a:_) (s:state a)
   (tag:Hacl.Hash.Definitions.hash_t a)
   (tx:G.erased transcript_t)
-  : ST unit
+  : Stack unit
     (requires (fun h0 ->
       let tx = G.reveal tx in
       invariant s tx h0 /\
@@ -387,11 +525,14 @@ val extract_hash
       B.as_seq h1 tag == Spec.Hash.hash a (transcript_bytes tx)))
 
 
-(*
-val free
-*)
-
-(* We need some form of collision resistance adapted to transcripts.
-   i.e., if the hashes of two transcripts match then the transcripts
-   themselves do.
-*)
+/// `injectivity`: The main lemma provided by this module is a form of
+///  collision resistance adapted to transcripts, i.e., if the hashes
+///  of two transcripts match then the transcripts themselves do.
+val injectivity (a:HashDef.hash_alg) (tx1 tx2:G.erased transcript_t)
+  : Lemma
+    (ensures (
+      let tx1 = G.reveal tx1 in
+      let tx2 = G.reveal tx2 in
+      Spec.Hash.hash a (transcript_bytes tx1) ==
+      Spec.Hash.hash a (transcript_bytes tx2) ==>
+      tx1 == tx2))
