src/tls/MITLS.Repr.Handshake.fst
@@ -1,4 +1,12 @@
 module MITLS.Repr.Handshake
+(* Summary:
+
+   This module encapsulates wire-format representations of
+   Parsers.Handshake messages.
+
+   Its main type, `repr b` is an instance of MITLS.Repr.repr
+   instantiated with serverHello_parser
+*)
 module LP = LowParse.Low.Base
 module B = LowStar.Monotonic.Buffer
 module HS = FStar.HyperStack
@@ -11,18 +19,10 @@ open FStar.HyperStack.ST
 
 let t = HSM.handshake
 
-let repr #p #q (b:LP.slice p q) =
+let repr (b:R.slice) =
   R.repr_p HSM.handshake b HSM.handshake_parser
 
-let mk #p #q (b:LP.slice p q) (from to:R.index b)
-  : Stack (repr b)
-    (requires R.valid_pos b HSM.handshake_parser from to)
-    (ensures fun h0 r h1 ->
-      B.modifies B.loc_none h0 h1 /\
-      R.valid r h1)
-  = R.mk b from to HSM.handshake_parser
-
-let handshakeType (#b:LP.slice 'p 'q) (r:repr b)
+let handshakeType (#b:R.slice) (r:repr b)
   : Stack Parsers.HandshakeType.handshakeType
     (requires
       R.valid r)
@@ -34,7 +34,7 @@ let handshakeType (#b:LP.slice 'p 'q) (r:repr b)
     R.reveal_valid();
     handshakeType_reader b r.start_pos
 
-let clientHello (#b:LP.slice 'p 'q) (r:repr b)
+let clientHello (#b:R.slice) (r:repr b)
   : Stack (RCH.repr b)
     (requires fun h ->
       R.valid r h /\
@@ -50,11 +50,11 @@ let clientHello (#b:LP.slice 'p 'q) (r:repr b)
     let pos' = HSM.handshake_accessor_client_hello b r.start_pos in
     assume (LP.valid Parsers.ClientHello.clientHello_parser h b pos');
     let end_pos = Parsers.ClientHello.clientHello_jumper b pos' in
-    let ch_repr = RCH.mk b pos' end_pos in
-    admit();
+    let ch_repr = R.mk b pos' end_pos Parsers.ClientHello.clientHello_parser in
+    assume (R.value ch_repr == HSM.M_client_hello?._0 (R.value r));
     ch_repr
 
-let serverHello (#b:LP.slice 'p 'q) (r:repr b)
+let serverHello (#b:R.slice) (r:repr b)
   : Stack (RSH.repr b)
     (requires fun h ->
       R.valid r h /\
@@ -70,6 +70,6 @@ let serverHello (#b:LP.slice 'p 'q) (r:repr b)
     let pos' = HSM.handshake_accessor_server_hello b r.start_pos in
     assume (LP.valid Parsers.ServerHello.serverHello_parser h b pos');
     let end_pos = Parsers.ServerHello.serverHello_jumper b pos' in
-    let sh_repr = RSH.mk b pos' end_pos in
-    admit();
+    let sh_repr = R.mk b pos' end_pos Parsers.ServerHello.serverHello_parser in
+    assume (R.value sh_repr == HSM.M_server_hello?._0 (R.value r));
     sh_repr
