src/tls/MITLS.Repr.fst
@@ -1,74 +1,150 @@
 module MITLS.Repr
+
+(* Summary:
+
+   This module provides the "base" type of several types that
+   encapsulate the wire-format representations of TLS messages.
+
+   Its main features are:
+
+   1. A type `repr t b`: Given a backing array of bytes `b`
+      (represented as a `slice` in the parlance of LowParse), `repr t
+      b` stands for a representation of `t`-typed values in `b`.
+
+   2. An abstract predicate `valid r h`, stating that memory state `h`
+      contains a valid representation `r`. This predicate comes with a
+      framing principle and SMT triggers for it.
+*)
 module LP = LowParse.Low.Base
 module B = LowStar.Monotonic.Buffer
 module HS = FStar.HyperStack
 open FStar.Integers
 
-let index (b:LP.slice 'p 'q) = i:uint_32{ i <= LP.(b.len) }
+(* For now, we restrict `repr` to only use mutable slices as its
+   backing u8 store.
 
-assume
-val rewritable (#p #q:_) (out:LP.slice p q) (from to:index out) (h:HS.mem) : prop
+   In the future, we may generalize this to support `const` slices,
+   i.e., reprs backed by a slice whose buffer is either mutable or
+   immutable.
+*)
 
+/// A wrapper around trivial preorders from LowStar.Buffer. The
+/// explicit erasure here is because LowParse is working around a
+/// known F* issue (#1694). It will eventually be removed.
+let trivial_preorder : LP.srel LP.byte =
+  Ghost.hide (LowStar.Buffer.trivial_preorder LP.byte)
+
+
+/// A mutable slice: Eventually, we might just change this one
+///   definition to be a const slice, multiplexing over mutable and
+///   immutable LP.slices
+let slice = LP.slice trivial_preorder trivial_preorder
+
+/// `index b` is the type of valid indexes into `b`
+let index (b:slice)= i:uint_32{ i <= LP.(b.len) }
+
+/// `strong_parser_kind`: We restrict our attention to the
+/// representation of types whose parsers have the strong-prefix
+/// property.
 let strong_parser_kind =
-    k:LP.parser_kind{LP.(k.parser_kind_subkind == Some ParserStrong)}
+    k:LP.parser_kind{
+      LP.(k.parser_kind_subkind == Some ParserStrong)
+    }
 
+(*** Representation types ***)
+
+/// `repr_meta t`: Each representation is associated with metadata
+/// that records both
+///  -- the parser that defines the wire-format used
+///  -- an erased value represented by the wire format
 noeq
 type repr_meta (t:Type) = {
   parser_kind: strong_parser_kind;
-  parser:LP.parser parser_kind t; //erased anyway
+  parser:LP.parser parser_kind t;
   value: t;
 }
 
+/// `repr t b`: The main type of this module.
+///
+///   * The slice `b` holds a representation of `t` in
+///    `b.[start_pos, end_pos)`
+///
+///   * The representation is described by erased the `meta` field
 noeq
-type repr #p #q (t:Type) (b:LP.slice p q) = {
+type repr (t:Type) (b:slice) = {
   start_pos: index b;
   end_pos: i:index b {start_pos <= i };
   meta: Ghost.erased (repr_meta t)
 }
 
 
-let value #p #q (#t:Type) (#b:LP.slice p q) (r:repr t b) 
-  : GTot t
-  = (Ghost.reveal r.meta).value
-  
-let repr_p #p #q (t:Type) (b:LP.slice p q) #k (parser:LP.parser k t) =
+/// `repr_p`
+///
+/// One of the main ideas of `repr` is to index representation by
+/// types rather than parsers that define wire-formats.
+///
+/// When manipulating reprs, the intention is for clients to be
+/// agnostic to the specific wire formats used.
+///
+/// Nevertheless, at various points, we need to construct
+/// representations from wire formats. At those points, the `repr_p`
+/// type is useful, since it is a `repr` that is also indexed by a
+/// parser.
+let repr_p (t:Type) (b:slice) #k (parser:LP.parser k t) =
   r:repr t b {
     let meta = Ghost.reveal r.meta in
     meta.parser_kind == k /\
     meta.parser == parser
   }
 
-let valid_pos #t #p #q (b:LP.slice p q)
-              #k (parser:LP.parser k t)
-              (from to:uint_32)
-              (h:HS.mem)
-  : prop
-  = LP.live_slice h b /\ //consequence of the next clause
-    LP.valid_pos parser h b from to
+(*** Validity ***)
 
-let valid' #t #p #q (#b:LP.slice p q) (r:repr t b) (h:HS.mem)
-  : prop
+/// `valid' r h`:
+///   We define validity in two stages:
+///
+///   First, we provide `valid'`, a transparent definition and then
+///   turn it `abstract` by the `valid` predicate just below.
+///
+///   Validity encapsulate two related LowParse notions:
+///
+///    1. That the underlying slice contains a valid wire-format
+///    (`valid_pos`)
+///
+///    2. That the ghost value associated with the `repr` is the
+///    parsed value of the wire format.
+///
+let valid' (#t:Type) (#b:slice) (r:repr t b) (h:HS.mem)
   = let m = Ghost.reveal r.meta in
-    valid_pos b m.parser r.start_pos r.end_pos h /\
+    LP.valid_pos m.parser h b r.start_pos r.end_pos /\
     m.value == LP.contents m.parser h b r.start_pos
 
+
+/// `valid`: abstract validity
 abstract
-let valid #t #p #q (#b:LP.slice p q) (r:repr t b) (h:HS.mem)
-  : prop
+let valid (#t:Type) (#b:slice) (r:repr t b) (h:HS.mem)
   = valid' r h
 
+
+/// `reveal_valid`:
+///   An explicit lemma exposes the definition of `valid`
 let reveal_valid ()
-  : Lemma (forall t p q (b:LP.slice p q) (r:repr t b) (h:HS.mem).
-              {:pattern (valid r h)}
-           valid r h <==> valid' r h)
+  : Lemma (forall (t:Type) (b:slice) (r:repr t b) (h:HS.mem).
+              {:pattern (valid #t #b r h)}
+           valid #t #b r h <==> valid' #t #b r h)
   = ()
-  
-let fp #t #p #q (#b:LP.slice p q) (r:repr t b) =
-  LP.loc_slice_from_to b r.start_pos r.end_pos
-  
-let frame_valid #t #p #q (#b:LP.slice p q) (r:repr t b) (l:B.loc) (h0 h1:HS.mem)
-  : Lemma 
-    (requires 
+
+/// `fp r`: The memory footprint of a repr is the
+///         sub-slice b.[from, to)
+let fp #t (#b:slice) (r:repr t b)
+  : GTot B.loc
+  = LP.loc_slice_from_to b r.start_pos r.end_pos
+
+/// `frame_valid`:
+///    A framing principle for `valid r h`
+///    It is invariant under footprint-preserving heap updates
+let frame_valid #t #b (r:repr t b) (l:B.loc) (h0 h1:HS.mem)
+  : Lemma
+    (requires
       valid r h0 /\
       B.modifies l h0 h1 /\
       B.loc_disjoint (fp r) l)
@@ -78,14 +154,29 @@ let frame_valid #t #p #q (#b:LP.slice p q) (r:repr t b) (l:B.loc) (h0 h1:HS.mem)
      SMTPat (B.modifies l h0 h1)]
   = B.modifies_buffer_from_to_elim LP.(b.base) r.start_pos r.end_pos l h0 h1
 
+
+/// `value`: A convenience function to access the underlying value
+/// represented
+let value #t #b (r:repr t b)
+  : GTot t
+  = (Ghost.reveal r.meta).value
+
 open FStar.HyperStack.ST
-let mk #p #q (b:LP.slice p q) (from to:index b)
+/// `mk b from to p`:
+///    Constructing a `repr` from a sub-slice
+///      b.[from, to)
+///    known to be valid for a given wire-format parser `p`
+let mk (b:slice) (from to:index b)
        (#k:strong_parser_kind) #t (parser:LP.parser k t)
   : Stack (repr_p t b parser)
-    (requires valid_pos b parser from to)
+    (requires fun h ->
+      LP.valid_pos parser h b from to)
     (ensures fun h0 r h1 ->
       B.modifies B.loc_none h0 h1 /\
-      valid r h1)
+      valid r h1 /\
+      r.start_pos = from /\
+      r.end_pos = to /\
+      value r == LP.contents parser h1 b from)
   = let h = get () in
     let m =
       let v = LP.contents parser h b from in
